\documentclass[12pt]{article}

% Set margins
\usepackage[margin=0.5in]{geometry}
% Remove paragraph indentation
\setlength{\parindent}{1\baselineskip}
\setlength{\parskip}{0.5\baselineskip}

\usepackage{amsmath}
\usepackage{amssymb}
\usepackage{amsfonts}
\usepackage{hyperref}
\usepackage{amsthm}
\usepackage{tikz-cd}
\usepackage{tikz}
\usepackage{cancel}
\usepackage{mdframed}
\usepackage{enumitem}
\usepackage{tikz-cd}
\usepackage{bm}

\begin{document}

\title{Physics 151 Pset Suggestions}
\date{\today}
\maketitle

\section{Pset 1}

Recall the Lagrangian vector from class (compact form and in components)
\[ 
    \begin{aligned}
        \mathbb L 
        &= \dfrac d {dt} \nabla_{\dot q} \mathcal L - \nabla_q \mathcal L \\ 
        \mathbb L_j 
        &= \dfrac d {dt} \partial_{\dot q_j} \mathcal L - \nabla_q \mathcal L 
    \end{aligned}
\] 
To emphasize dependence on $q$ (or $x$), we occasionally write 
\[\begin{aligned}
    \mathbb L_q &= \dfrac d {dt} \nabla_{\dot q} \mathcal L - \nabla_q \mathcal L \\ 
    \mathbb L_x &= \dfrac d {dt} \nabla_{\dot x} \mathcal L - \nabla_x \mathcal L \\ 
\end{aligned}\] 
Also recall that the Jacobian matrix $J_{a\to b}$ from $a\in {\mathbb R}^m$ to $b\in {\mathbb R}^n$ is 
\[ 
    (J_{a\to b})_{ij} = \begin{bmatrix}
        \nabla_a b_1 & \cdots & \nabla_a b_n 
    \end{bmatrix} = \dfrac{\partial b_j}{\partial a_i}
\] 
so that the chain rule can be written as (compactly and in components) 
\[ 
    \begin{aligned}
        \nabla_a f(b) &= J_{a\to b} \nabla_b f(b)\\ 
        \dfrac{\partial}{\partial a_j} f(b(a_1, \cdots, a_m)) &= 
        \sum_k \dfrac{\partial f(b)}{\partial b_k} \dfrac{\partial b_k}{\partial a_j}
        = \sum_k (J_{a\to b})_{jk} (\nabla_b f(b))_k 
    \end{aligned}
\] 
This question asks you to show that the Lagrangian 
vector transforms covariantly:
\begin{enumerate}[label=(\alph*), topsep=0pt]
    \item Given a coordinate transform $x\to q$ so that $q_j=q_j(x_1, \cdots, x_n)$, 
    it determines a transform $(x, \dot x)\to (q, \dot q)$ of the derivatives as well. 
    Show that $J_{\dot x\to \dot q} = J_{x\to q}$. 
    
    \textit{Hint: the transformation $x\to q$ is independent of $\dot x$, 
    so one can show that $\dot x, \dot q$ are related by a linear transform 
    $\dot q = J_{x\to q}\dot x$ or, in components, 
    $\dot q_j = \sum_k (J_{x\to q})_{jk} \dot x_k$}. 

    \item Show that $J_{x\to \dot q} = \dfrac d {dt} J_{x\to q}$. 
    \item Explain why $J_{\dot x\to q}=0$. 
    \item The previous parts give us the full Jacobian of $(x, \dot x)\to (q, \dot q)$ 
    \[  
        J_{(x, \dot x)\to (q, \dot q)} = \begin{bmatrix}
            J_{x\to q} & J_{x\to \dot q} \\ 
            J_{\dot x\to q} & J_{\dot x\to \dot q} 
        \end{bmatrix} = \begin{bmatrix}
            J_{x\to q} & \dfrac d {dt} J_{x\to q} \\ 0 & J_{x\to q}
        \end{bmatrix}
    \] 
    Next show that $\nabla_{\dot x} \mathbb L_q = J_{\dot x\to \dot q}\nabla_{\dot q}$ 
    \item Show that 
    $\nabla_x \mathbb L = \left(J_{x\to q}\nabla_q + J_{x\to \dot q}\nabla_{\dot q}\right)\mathbb L$ 
    \item Covariance follows from the previous parts: show that $\mathbb L_x = J_{x\to q}\mathbb L_q$. 
\end{enumerate}


\subsection{Solutions}
\begin{enumerate}[label=(\alph*), topsep=0pt]
    \item By the chain rule
    \[ 
        \dot q_j = \dfrac d {dt} q_j(x) 
        = \sum_k \dfrac{\partial q_j}{\partial x_k} \dfrac d {dt} x_k = (J_{x\to q})_{kj}\dot x_k 
    \] 
\end{enumerate}

\end{document}